trying to prove that the rust version of is_elem satisfies its functional specification

heapster-saw/examples/rust_data_proofs.v
@@ -22,6 +22,45 @@ Proof.
   time "no_errors_is_elem" prove_refinement.
 Qed.
 
+Definition is_elem_fun' : bitvector 64 -> List_IRT (bitvector 64) ->
+                          CompM (unit * bitvector 1) :=
+  multiArgFixM
+    (LRT_Fun (bitvector 64)
+             (fun _ => LRT_Fun _ (fun _ => LRT_Ret (unit * bitvector 1))))
+    (fun is_elem x l =>
+       either
+         _ _ _
+         (fun _ => returnM (tt, intToBv 1 0))
+         (fun arg =>
+            let y := fst (snd arg) in
+            let l' := fst (snd (snd arg)) in
+            if bvEq 64 y x then returnM (tt, intToBv 1 1) else is_elem x l')
+         (unfoldList_IRT _ l)).
+
+Definition is_elem_fun : bitvector 64 -> List_IRT (bitvector 64) ->
+                         CompM (unit * bitvector 1) :=
+  fst
+    (multiFixM
+       (lrts := LRT_Cons (LRT_Fun _ (fun _ => LRT_Fun _ (fun _ => LRT_Ret _))) LRT_Nil)
+       (fun is_elem =>
+          (fun x l =>
+             either
+               _ _ _
+               (fun _ => returnM (tt, intToBv 1 0))
+               (fun arg =>
+                  let y := fst (snd arg) in
+                  let l' := fst (snd (snd arg)) in
+                  if bvEq 64 y x then returnM (tt, intToBv 1 1) else is_elem x l')
+               (unfoldList_IRT _ l), tt))).
+
+Lemma is_elem_fun_ref : refinesFun is_elem is_elem_fun.
+Proof.
+  unfold is_elem, is_elem__tuple_fun, noErrorsSpec,
+         list_64_drop_in_place, _ZN5alloc5alloc8box_free17hc52ecccd139e11ceE,
+         llvm__x2ememcpy__x2ep0i8__x2ep0i8__x2ei64, is_elem_fun.
+  time "is_elem_fun_ref" prove_refinement.
+Admitted.
+
 
 (* Print bool_and__tuple_fun. *)
 
